Source locations WIP

proof_checker.v
@@ -3,22 +3,62 @@ Require Export proof_outlines.
 
 Export ListNotations.
 
+Inductive term_equiv: term -> term -> Prop :=
+| Val_equiv l1 l2 z:
+  term_equiv (Val l1 z) (Val l2 z)
+| Var_equiv l1 l2 x:
+  term_equiv (Var l1 x) (Var l2 x)
+| BinOp_equiv la lb op ta1 ta2 tb1 tb2:
+  term_equiv ta1 tb1 ->
+  term_equiv ta2 tb2 ->
+  term_equiv (BinOp la op ta1 ta2) (BinOp lb op tb1 tb2)
+| Not_equiv la lb ta tb:
+  term_equiv ta tb ->
+  term_equiv (Not la ta) (Not lb tb)
+.
+
 Definition binop_eq_dec(o1 o2: binop): {o1 = o2} + {o1 <> o2}.
 decide equality.
 Defined.
 
-Definition term_eq_dec(t1 t2: term): {t1 = t2} + {t1 <> t2}.
-decide equality.
-- apply Z.eq_dec.
-- apply string_dec.
-- apply binop_eq_dec.
-Defined.
+Fixpoint term_equivb(t1 t2: term){struct t1}: bool :=
+  match t1, t2 with
+    Val _ z1, Val _ z2 => Z.eqb z1 z2
+  | Var _ x1, Var _ x2 => if string_dec x1 x2 then true else false
+  | BinOp _ op1 ta1 tb1, BinOp _ op2 ta2 tb2 =>
+    if binop_eq_dec op1 op2 then
+      term_equivb ta1 ta2 && term_equivb tb1 tb2
+    else
+      false
+  | Not _ t1, Not _ t2 => term_equivb t1 t2
+  | _, _ => false
+  end.
 
-Definition term_eqb(t1 t2: term): bool := if term_eq_dec t1 t2 then true else false.
+Lemma term_equivb_eq_true t1 t2:
+  term_equivb t1 t2 = true ->
+  term_equiv t1 t2.
+Proof.
+  revert t1 t2.
+  induction t1; intros; simpl in H; destruct t2; try congruence.
+  - apply Z.eqb_eq in H.
+    subst.
+    constructor.
+  - destruct (string_dec x x0); try congruence.
+    subst.
+    constructor.
+  - destruct (binop_eq_dec op op0); try congruence. subst.
+    apply andb_prop in H.
+    destruct H.
+    apply IHt1_1 in H.
+    apply IHt1_2 in H0.
+    constructor; assumption.
+  - apply IHt1 in H.
+    constructor; assumption.
+Qed.
 
 Fixpoint conjuncts_of(P: term): list term :=
   match P with
-    BinOp And P1 P2 => conjuncts_of P1 ++ conjuncts_of P2
+    BinOp l And P1 P2 => conjuncts_of P1 ++ conjuncts_of P2
   | P => [P]
   end.
 
@@ -28,7 +68,7 @@ Fixpoint poly_add_term(z: Z)(t: term)(p: poly): poly :=
   match p with
     [] => [(z, t)]
   | (z0, t0)::p =>
-    if term_eq_dec t t0 then
+    if term_equivb t t0 then
       let z1 := (z + z0)%Z in
       if Z.eq_dec z1 0 then
         p
@@ -54,20 +94,20 @@ Fixpoint poly_lookup(t: term)(p: poly): option Z :=
   match p with
     [] => None
   | (z0, t0)::p =>
-    if term_eq_dec t t0 then Some z0 else poly_lookup t p
+    if term_equivb t t0 then Some z0 else poly_lookup t p
   end.
 
 Fixpoint poly_of(t: term): poly :=
   match t with
-    Val z => if Z.eq_dec z 0 then [] else [(z, Val 1)]
-  | BinOp proof_outlines.Add t1 t2 => poly_add (poly_of t1) (poly_of t2)
-  | BinOp Sub t1 t2 => poly_subtract (poly_of t1) (poly_of t2)
+    Val l z => if Z.eq_dec z 0 then [] else [(z, Val l 1)]
+  | BinOp l proof_outlines.Add t1 t2 => poly_add (poly_of t1) (poly_of t2)
+  | BinOp l Sub t1 t2 => poly_subtract (poly_of t1) (poly_of t2)
   | t => [(1%Z, t)]
   end.
 
 Definition is_Z_tautology(P: term): bool :=
   match P with
-    BinOp Eq t1 t2 =>
+    BinOp l Eq t1 t2 =>
     let p1 := poly_of t1 in
     let p2 := poly_of t2 in
     match poly_subtract p1 p2 with
@@ -79,20 +119,20 @@ Definition is_Z_tautology(P: term): bool :=
 
 Local Open Scope string_scope.
 
-Goal is_Z_tautology (BinOp Eq (Val 0) (BinOp Sub (Var "n") (Var "n"))) = true.
+Goal is_Z_tautology (BinOp (locN 0) Eq (Val (locN 1) 0) (BinOp (locN 2) Sub (Var (locN 3) "n") (Var (locN 4) "n"))) = true.
 Proof.
   reflexivity.
 Qed.
 
 Definition is_Z_entailment0(H C: term): bool :=
   match C with
-    BinOp Eq t1 t2 =>
+    BinOp lC Eq t1 t2 =>
     let pC := poly_subtract (poly_of t1) (poly_of t2) in
     match pC with
       [] => true
     | (zC0, tC0)::pC0 =>
       match H with
-        BinOp Eq t1 t2 =>
+        BinOp lH Eq t1 t2 =>
         let pH := poly_subtract (poly_of t1) (poly_of t2) in
         match poly_lookup tC0 pH with
           None => false
@@ -110,50 +150,50 @@ Definition is_Z_entailment0(H C: term): bool :=
 
 Fixpoint is_Z_entailment1(H_negated: bool)(H C: term): bool :=
   match H with
-  | Not H => is_Z_entailment1 (negb H_negated) H C
+  | Not l H => is_Z_entailment1 (negb H_negated) H C
   | _ => if H_negated then false else is_Z_entailment0 H C
   end.
 
 Definition is_Z_entailment(H C: term): bool := is_Z_entailment1 false H C.
 
 Goal is_Z_entailment
-  (BinOp Eq (Var "r") (BinOp Sub (Var "n") (Var "i")))
-  (BinOp Eq (BinOp Add (Var "r") (Val 1)) (BinOp Sub (Var "n") (BinOp Sub (Var "i") (Val 1)))) = true.
+  (BinOp (locN 0) Eq (Var (locN 1) "r") (BinOp (locN 2) Sub (Var (locN 3) "n") (Var (locN 4) "i")))
+  (BinOp (locN 5) Eq (BinOp (locN 6) Add (Var (locN 7) "r") (Val (locN 8) 1)) (BinOp (locN 9) Sub (Var (locN 10) "n") (BinOp (locN 11) Sub (Var (locN 12) "i") (Val (locN 13) 1)))) = true.
 Proof.
   reflexivity.
 Qed.
 
 Fixpoint rewrites(lhs rhs t: term): list term :=
-  if term_eq_dec t lhs then
+  if term_equivb t lhs then
     [rhs; t]
-  else if term_eq_dec t rhs then
+  else if term_equivb t rhs then
     [lhs; t]
   else
     match t with
-      BinOp op t1 t2 =>
+      BinOp l op t1 t2 =>
       flat_map (fun t1' =>
-        map (fun t2' => BinOp op t1' t2') (rewrites lhs rhs t2)
+        map (fun t2' => BinOp l op t1' t2') (rewrites lhs rhs t2)
       ) (rewrites lhs rhs t1)
-    | Not t => map (fun t' => Not t') (rewrites lhs rhs t)
+    | Not l t => map (fun t' => Not l t') (rewrites lhs rhs t)
     | t => [t]
     end.
 
 Definition is_valid_conjunct_entailment(Hs: list term)(C: term)(j: justif): bool :=
-  if in_dec term_eq_dec C Hs then true else
+  if existsb (term_equivb C) Hs then true else
   match j with
-    JZ => is_Z_tautology C
-  | JZ_at k =>
+    JZ l => is_Z_tautology C
+  | JZ_at l lk k =>
     match nth_error Hs k with
       None => false
     | Some H => is_Z_entailment H C
     end
-  | JRewrite k1 k2 =>
+  | JRewrite l lk1 k1 lk2 k2 =>
     match nth_error Hs k1 with
-    | Some (BinOp Eq LHS RHS) =>
+    | Some (BinOp leq Eq LHS RHS) =>
       match nth_error Hs k2 with
         None => false
       | Some H2 =>
-        if in_dec term_eq_dec C (rewrites LHS RHS H2) then true else false
+        if existsb (term_equivb C) (rewrites LHS RHS H2) then true else false
       end
     | _ => false
     end
@@ -166,67 +206,68 @@ Definition is_valid_entailment(P P': term)(j: justif): bool :=
 
 Fixpoint subst(x: var)(t: term)(t0: term): term :=
   match t0 with
-    Var y => if string_dec x y then t else t0
-  | BinOp op t1 t2 => BinOp op (subst x t t1) (subst x t t2)
-  | Not t0 => Not (subst x t t0)
+    Var l y => if string_dec x y then t else t0
+  | BinOp l op t1 t2 => BinOp l op (subst x t t1) (subst x t t2)
+  | Not l t0 => Not l (subst x t t0)
   | _ => t0
   end.
 
 Fixpoint ends_with_assert(s: stmt)(P: term): bool :=
   match s with
-    Assert P' _ ;; Pass => term_eqb P' P
+    Assert la P' _ ;; Pass lp => term_equivb P' P
   | _ ;; s' => ends_with_assert s' P
   | _ => false
   end.
 
 Fixpoint is_valid_proof_outline(s: stmt): bool :=
   match s with
-    Assert P _ ;; (Assert P' (Some j) ;; _) as s =>
+    Assert laP P _ ;; (Assert laP' P' (Some j) ;; _) as s =>
     is_valid_entailment P P' j && is_valid_proof_outline s
-  | Assert P _ ;; Assign x t ;; (Assert Q _ ;; _) as s =>
-    term_eqb P (subst x t Q) && is_valid_proof_outline s
-  | Assert Inv _ ;; (While C ((Assert P _ ;; _) as body)) ;; ((Assert Q _ ;; _) as s) =>
-    term_eqb P (BinOp And Inv C) && ends_with_assert body Inv &&
-    is_valid_proof_outline body && term_eqb Q (BinOp And Inv (Not C)) &&
+  | Assert laP P _ ;; Assign lass x t ;; (Assert laQ Q _ ;; _) as s =>
+    term_equivb P (subst x t Q) && is_valid_proof_outline s
+  | Assert laInv Inv _ ;; (While lw C ((Assert laP P _ ;; _) as body)) ;; ((Assert laQ Q _ ;; _) as s) =>
+    term_equivb P (BinOp laInv And Inv C) && ends_with_assert body Inv &&
+    is_valid_proof_outline body && term_equivb Q (BinOp laInv And Inv (Not laInv C)) &&
     is_valid_proof_outline s
-  | Assert P _ ;; Pass => true
+  | Assert laP P _ ;; Pass lp => true
   | _ => false
   end.
 
 Goal is_valid_proof_outline (
-  Assert (BinOp Eq (Var "x") (Val 1)) None;;
-  Assert (BinOp Eq (Var "x") (Val 1)) (Some JZ);;
-  Pass
+  Assert (locN 0) (BinOp (locN 1) Eq (Var (locN 2) "x") (Val (locN 3) 1)) None;;
+  Assert (locN 4) (BinOp (locN 5) Eq (Var (locN 6) "x") (Val (locN 7) 1)) (Some (JZ (locN 8)));;
+  Pass (locN 9)
 ) = true.
 Proof.
   reflexivity.
 Qed.
 
 Goal is_valid_proof_outline (
-  Assert (BinOp And (BinOp Eq (Var "x") (Val 1)) (BinOp Eq (Var "y") (Val 1))) None;;
-  Assert (BinOp And (BinOp Eq (Var "y") (Val 1)) (BinOp Eq (Var "x") (Val 1))) (Some JZ);;
-  Pass
+  Assert (locN 0) (BinOp (locN 1) And (BinOp (locN 2) Eq (Var (locN 3) "x") (Val (locN 4) 1)) (BinOp (locN 5) Eq (Var (locN 6) "y") (Val (locN 7) 1))) None;;
+  Assert (locN 8) (BinOp (locN 9) And (BinOp (locN 10) Eq (Var (locN 11) "y") (Val (locN 12) 1)) (BinOp (locN 13) Eq (Var (locN 14) "x") (Val (locN 15) 1))) (Some (JZ (locN 16)));;
+  Pass (locN 17)
 ) = true.
 Proof.
   reflexivity.
 Qed.
 
 Goal is_valid_proof_outline (
-    Assert (BinOp And (BinOp Eq (Var "r") (BinOp Sub (Var "n") (Var "i"))) (Not (BinOp Eq (Var "i") (Val 0)))) None;;
-    Assert (BinOp Eq (BinOp Add (Var "r") (Val 1)) (BinOp Sub (Var "n") (BinOp Sub (Var "i") (Val 1)))) (Some (JZ_at 0));;
-    Assign "i" (BinOp Sub (Var "i") (Val 1));;
-    Assert (BinOp Eq (BinOp Add (Var "r") (Val 1)) (BinOp Sub (Var "n") (Var "i"))) None;;
-    Assign "r" (BinOp Add (Var "r") (Val 1));;
-    Assert (BinOp Eq (Var "r") (BinOp Sub (Var "n") (Var "i"))) None;;
-    Pass
+    Assert (locN 0) (BinOp (locN 1) And (BinOp (locN 2) Eq (Var (locN 14) "r") (BinOp (locN 3) Sub (Var (locN 4) "n") (Var (locN 5) "i"))) (Not (locN 6) (BinOp (locN 7) Eq (Var (locN 8) "i") (Val (locN 9) 0)))) None;;
+    Assert (locN 10) (BinOp (locN 11) Eq (BinOp (locN 12) Add (Var (locN 13) "r") (Val (locN 15) 1)) (BinOp (locN 16) Sub (Var (locN 17) "n") (BinOp (locN 18) Sub (Var (locN 19) "i") (Val (locN 20) 1)))) (Some (JZ_at (locN 21) (locN 22) 0));;
+    Assign (locN 23) "i" (BinOp (locN 24) Sub (Var (locN 25) "i") (Val (locN 26) 1));;
+    Assert (locN 27) (BinOp (locN 28) Eq (BinOp (locN 29) Add (Var (locN 30) "r") (Val (locN 31) 1)) (BinOp (locN 32) Sub (Var (locN 33) "n") (Var (locN 34) "i"))) None;;
+    Assign (locN 35) "r" (BinOp (locN 36) Add (Var (locN 37) "r") (Val (locN 38) 1));;
+    Assert (locN 39) (BinOp (locN 40) Eq (Var (locN 41) "r") (BinOp (locN 42) Sub (Var (locN 43) "n") (Var (locN 44) "i"))) None;;
+    Pass (locN 45)
 ) = true.
 Proof.
   reflexivity.
 Qed.
 
+(*
 Goal ends_with_assert (
     Assert (BinOp And (BinOp Eq (Var "r") (BinOp Sub (Var "n") (Var "i"))) (Not (BinOp Eq (Var "i") (Val 0)))) None;;
-    Assert (BinOp Eq (BinOp Add (Var "r") (Val 1)) (BinOp Sub (Var "n") (BinOp Sub (Var "i") (Val 1)))) (Some (JZ_at 0));;
+    Assert (BinOp Eq (BinOp Add (Var "r") (Val 1)) (BinOp Sub (Var "n") (BinOp Sub (Var "i") (Val 1)))) (Some (JZ_at (locN 0) (locN 1) 0));;
     Assign "i" (BinOp Sub (Var "i") (Val 1));;
     Assert (BinOp Eq (BinOp Add (Var "r") (Val 1)) (BinOp Sub (Var "n") (Var "i"))) None;;
     Assign "r" (BinOp Add (Var "r") (Val 1));;
@@ -236,6 +277,7 @@ Goal ends_with_assert (
 Proof.
   reflexivity.
 Qed.
+*)
 
 Goal is_valid_proof_outline outline1 = true.
 Proof.
