semantics.v
@@ -8,60 +8,60 @@ Inductive value :=
 .
 
 Inductive evaluates_to(S: state): term -> value -> Prop :=
-| Val_evaluates_to z:
-  evaluates_to S (Val z) (VInt z)
-| Var_evaluates_to x z:
+| Val_evaluates_to l z:
+  evaluates_to S (Val l z) (VInt z)
+| Var_evaluates_to l x z:
   S x = Some z ->
-  evaluates_to S (Var x) (VInt z)
-| Add_evaluates_to t1 t2 z1 z2:
+  evaluates_to S (Var l x) (VInt z)
+| Add_evaluates_to l t1 t2 z1 z2:
   evaluates_to S t1 (VInt z1) ->
   evaluates_to S t2 (VInt z2) ->
-  evaluates_to S (BinOp Add t1 t2) (VInt (z1 + z2))
-| Sub_evaluates_to t1 t2 z1 z2:
+  evaluates_to S (BinOp l Add t1 t2) (VInt (z1 + z2))
+| Sub_evaluates_to l t1 t2 z1 z2:
   evaluates_to S t1 (VInt z1) ->
   evaluates_to S t2 (VInt z2) ->
-  evaluates_to S (BinOp Sub t1 t2) (VInt (z1 - z2))
-| Eq_evaluates_to_true t1 t2 v:
+  evaluates_to S (BinOp l Sub t1 t2) (VInt (z1 - z2))
+| Eq_evaluates_to_true l t1 t2 v:
   evaluates_to S t1 v ->
   evaluates_to S t2 v ->
-  evaluates_to S (BinOp Eq t1 t2) (VBool true)
-| Eq_evaluates_to_false t1 t2 v1 v2:
+  evaluates_to S (BinOp l Eq t1 t2) (VBool true)
+| Eq_evaluates_to_false l t1 t2 v1 v2:
   evaluates_to S t1 v1 ->
   evaluates_to S t2 v2 ->
   v1 <> v2 ->
-  evaluates_to S (BinOp Eq t1 t2) (VBool false)
-| And_evaluates_to t1 b1 t2 b2:
+  evaluates_to S (BinOp l Eq t1 t2) (VBool false)
+| And_evaluates_to l t1 b1 t2 b2:
   evaluates_to S t1 (VBool b1) ->
   evaluates_to S t2 (VBool b2) ->
-  evaluates_to S (BinOp And t1 t2) (VBool (b1 && b2))
-| Not_evaluates_to t b:
+  evaluates_to S (BinOp l And t1 t2) (VBool (b1 && b2))
+| Not_evaluates_to l t b:
   evaluates_to S t (VBool b) ->
-  evaluates_to S (Not t) (VBool (negb b))
+  evaluates_to S (Not l t) (VBool (negb b))
 .
 
 Definition update(x: var)(z: Z)(S: state): state :=
   fun y => if string_dec x y then Some z else S y.
 
 Inductive terminates_in: state -> stmt -> state -> Prop :=
-| Assert_terminates_in S P j:
+| Assert_terminates_in S l P j:
   evaluates_to S P (VBool true) ->
-  terminates_in S (Assert P j) S
-| Assign_terminates_in S x t z:
+  terminates_in S (Assert l P j) S
+| Assign_terminates_in S l x t z:
   evaluates_to S t (VInt z) ->
-  terminates_in S (Assign x t) (update x z S)
-| Pass_terminates_in S:
-  terminates_in S Pass S
+  terminates_in S (Assign l x t) (update x z S)
+| Pass_terminates_in S l:
+  terminates_in S (Pass l) S
 | Seq_terminates_in S s1 S' s2 S'':
   terminates_in S s1 S' ->
   terminates_in S' s2 S'' ->
   terminates_in S (s1 ;; s2) S''
-| If_terminates_in S C b s1 s2 S':
+| If_terminates_in S C l b s1 s2 S':
   evaluates_to S C (VBool b) ->
   terminates_in S (if b then s1 else s2) S' ->
-  terminates_in S (If C s1 s2) S'
-| While_terminates_in S C s S':
-  terminates_in S (If C (s ;; While C s) Pass) S' ->
-  terminates_in S (While C s) S'
+  terminates_in S (If l C s1 s2) S'
+| While_terminates_in S l C s S':
+  terminates_in S (If l C (s ;; While l C s) (Pass l)) S' ->
+  terminates_in S (While l C s) S'
 .
 
 CoInductive diverges: state -> stmt -> Prop :=
@@ -72,11 +72,11 @@ CoInductive diverges: state -> stmt -> Prop :=
   terminates_in S s1 S' ->
   diverges S' s2 ->
   diverges S (s1 ;; s2)
-| If_diverges S C s1 s2 b:
+| If_diverges S l C s1 s2 b:
   evaluates_to S C (VBool b) ->
   diverges S (if b then s1 else s2) ->
-  diverges S (If C s1 s2)
-| While_diverges S C s:
-  diverges S (If C (s ;; While C s) Pass) ->
-  diverges S (While C s)
+  diverges S (If l C s1 s2)
+| While_diverges S l C s:
+  diverges S (If l C (s ;; While l C s) (Pass l)) ->
+  diverges S (While l C s)
 .
